thys/Native_Word/Uint.thy
@@ -676,6 +676,7 @@ global_interpretation uint: word_type_copy_target_language Abs_uint Rep_uint sig
     and uint_shiftl = uint.shiftl
     and uint_shiftr = uint.shiftr
     and uint_sshiftr = uint.sshiftr
+    and uint_set_bit = uint.set_bit
   by standard (simp_all add: wivs_index_def)
 
 code_printing constant uint_test_bit \<rightharpoonup>
@@ -685,23 +686,6 @@ code_printing constant uint_test_bit \<rightharpoonup>
   (Haskell) "Data'_Bits.testBitBounded" and
   (OCaml) "Uint.test'_bit" and
   (Scala) "Uint.test'_bit"
-
-definition uint_set_bit :: "uint \<Rightarrow> integer \<Rightarrow> bool \<Rightarrow> uint"
-where [code del]:
-  "uint_set_bit x n b =
-  (if n < 0 \<or> dflt_size_integer \<le> n then undefined (set_bit :: uint \<Rightarrow> _) x n b
-   else set_bit x (nat_of_integer n) b)"
-
-lemma set_bit_uint_code [code]:
-  "set_bit x n b = (if n < dflt_size then uint_set_bit x (integer_of_nat n) b else x)"
-  including undefined_transfer integer.lifting unfolding uint_set_bit_def
-  by (transfer) (auto cong: conj_cong simp add: not_less set_bit_beyond word_size)
-
-lemma uint_set_bit_code [code]:
-  "Rep_uint (uint_set_bit w n b) = 
-  (if n < 0 \<or> dflt_size_integer \<le> n then Rep_uint (undefined (set_bit :: uint \<Rightarrow> _) w n b)
-   else set_bit (Rep_uint w) (nat_of_integer n) b)"
-including undefined_transfer integer.lifting unfolding uint_set_bit_def by transfer simp
 
 code_printing constant uint_set_bit \<rightharpoonup>
   (SML) "Uint.set'_bit" and
