thys/Native_Word/Uint32.thy
@@ -500,6 +500,7 @@ global_interpretation uint32: word_type_copy_target_language Abs_uint32 Rep_uint
     and uint32_shiftl = uint32.shiftl
     and uint32_shiftr = uint32.shiftr
     and uint32_sshiftr = uint32.sshiftr
+    and uint32_set_bit = uint32.set_bit
   by standard simp_all
 
 code_printing constant uint32_test_bit \<rightharpoonup>
@@ -508,23 +509,6 @@ code_printing constant uint32_test_bit \<rightharpoonup>
   (OCaml) "Uint32.test'_bit" and
   (Scala) "Uint32.test'_bit" and
   (Eval) "(fn w => fn n => if n < 0 orelse 32 <= n then raise (Fail \"argument to uint32'_test'_bit out of bounds\") else Uint32.test'_bit w n)"
-
-definition uint32_set_bit :: "uint32 \<Rightarrow> integer \<Rightarrow> bool \<Rightarrow> uint32"
-where [code del]:
-  "uint32_set_bit x n b =
-  (if n < 0 \<or> 31 < n then undefined (set_bit :: uint32 \<Rightarrow> _) x n b
-   else set_bit x (nat_of_integer n) b)"
-
-lemma set_bit_uint32_code [code]:
-  "set_bit x n b = (if n < 32 then uint32_set_bit x (integer_of_nat n) b else x)"
-including undefined_transfer integer.lifting unfolding uint32_set_bit_def
-by(transfer)(auto cong: conj_cong simp add: not_less set_bit_beyond word_size)
-
-lemma uint32_set_bit_code [code]:
-  "Rep_uint32 (uint32_set_bit w n b) = 
-  (if n < 0 \<or> 31 < n then Rep_uint32 (undefined (set_bit :: uint32 \<Rightarrow> _) w n b)
-   else set_bit (Rep_uint32 w) (nat_of_integer n) b)"
-including undefined_transfer unfolding uint32_set_bit_def by transfer simp
 
 code_printing constant uint32_set_bit \<rightharpoonup>
   (SML) "Uint32.set'_bit" and
