thys/Native_Word/Uint64.thy
@@ -698,6 +698,7 @@ global_interpretation uint64: word_type_copy_target_language Abs_uint64 Rep_uint
     and uint64_shiftl = uint64.shiftl
     and uint64_shiftr = uint64.shiftr
     and uint64_sshiftr = uint64.sshiftr
+    and uint64_set_bit = uint64.set_bit
   by standard simp_all
 
 code_printing constant uint64_test_bit \<rightharpoonup>
@@ -706,23 +707,6 @@ code_printing constant uint64_test_bit \<rightharpoonup>
   (OCaml) "Uint64.test'_bit" and
   (Scala) "Uint64.test'_bit" and
   (Eval) "(fn x => fn i => if i < 0 orelse i >= 64 then raise (Fail \"argument to uint64'_test'_bit out of bounds\") else Uint64.test'_bit x i)"
-
-definition uint64_set_bit :: "uint64 \<Rightarrow> integer \<Rightarrow> bool \<Rightarrow> uint64"
-where [code del]:
-  "uint64_set_bit x n b =
-  (if n < 0 \<or> 63 < n then undefined (set_bit :: uint64 \<Rightarrow> _) x n b
-   else set_bit x (nat_of_integer n) b)"
-
-lemma set_bit_uint64_code [code]:
-  "set_bit x n b = (if n < 64 then uint64_set_bit x (integer_of_nat n) b else x)"
-including undefined_transfer integer.lifting unfolding uint64_set_bit_def
-by(transfer)(auto cong: conj_cong simp add: not_less set_bit_beyond word_size)
-
-lemma uint64_set_bit_code [code]:
-  "Rep_uint64 (uint64_set_bit w n b) = 
-  (if n < 0 \<or> 63 < n then Rep_uint64 (undefined (set_bit :: uint64 \<Rightarrow> _) w n b)
-   else set_bit (Rep_uint64 w) (nat_of_integer n) b)"
-including undefined_transfer unfolding uint64_set_bit_def by transfer simp
 
 code_printing constant uint64_set_bit \<rightharpoonup>
   (SML) "Uint64.set'_bit" and
